src/AsyncFinish/Find.v
@@ -1,0 +1,271 @@
+Require Import Coq.Lists.List.
+
+Require Import Aniceto.List.
+
+Require Import HJ.AsyncFinish.Lang.
+
+Section Find.
+  Variable check: finish -> bool.
+  
+  Fixpoint get_children (f:finish) : list finish :=
+  match f with
+  | Node l =>
+    (fix aux (l:list l_task) :=
+      match l with
+      | ((t, Blocked f') :: l) => f' :: (aux l)
+      | (t, Ready) :: l => aux l
+      | nil => nil
+      end) l
+  end.
+
+  Lemma get_children_rw_cons_ready:
+    forall t l,
+    get_children (Node ((t, Ready) :: l)) = get_children (Node l).
+  Proof.
+    intros.
+    simpl.
+    auto.
+  Qed.
+
+  Lemma get_children_rw_cons_blocked:
+    forall t f l,
+    get_children (Node ((t, Blocked f) :: l)) = f :: get_children (Node l).
+  Proof.
+    intros.
+    simpl.
+    auto.
+  Qed.
+
+  Fixpoint size (f:finish) := 
+  S (
+  match f with
+  | Node l =>
+    (fix aux (l:list l_task) :=
+      match l with
+      | cons (t, Blocked f') l => S (size f') + aux l
+      | cons (t, Ready) l => S (aux l)
+      | nil => 0
+      end
+    ) l
+  end).
+
+  Lemma size_rw_cons_ready:
+    forall t l,
+    size (Node ((t, Ready) :: l)) = S (size (Node l)).
+  Proof.
+    intros.
+    simpl.
+    auto.
+  Qed.
+
+  Lemma size_rw_cons_blocked:
+    forall t f l,
+    size (Node ((t, Blocked f) :: l)) = S (size f) + size (Node l).
+  Proof.
+    intros; simpl; auto.
+  Qed.
+
+  Definition l_size (l:list finish) : nat := summation size l.
+
+  Definition is_nil {A} (l:list A) : bool :=
+  match l with
+  | nil => true
+  | _ => false
+  end.
+
+  Let summation_size_get_children:
+    forall f,
+    summation size (get_children f) < size f.
+  Proof.
+    intros.
+    induction f using finish_ind_strong.
+    - compute. auto.
+    - rewrite get_children_rw_cons_ready.
+      rewrite size_rw_cons_ready.
+      auto with *.
+    - rewrite get_children_rw_cons_blocked.
+      rewrite summation_rw_cons.
+      rewrite size_rw_cons_blocked.
+      auto with *.
+  Qed.
+
+  Let summation_flat_map:
+    forall l,
+    summation size (flat_map get_children l) <= summation size l.
+  Proof.
+    induction l.
+    { auto. }
+    simpl.
+    rewrite summation_rw_cons.
+    rewrite summation_rw_app.
+    assert (summation size (get_children a) < size a) by auto using summation_size_get_children.
+    auto with *.
+  Qed.
+
+  Lemma l_size_children_not_nil:
+    forall l,
+    is_nil (flat_map get_children l) = false ->
+    l_size (flat_map get_children l) < l_size l.
+  Proof.
+    intros.
+    induction l.
+    { inversion H. }
+    simpl.
+    simpl.
+    unfold l_size.
+    rewrite summation_rw_cons.
+    rewrite summation_rw_app.
+    assert (summation size (get_children a) < size a) by auto using summation_size_get_children.
+    assert (summation size (flat_map get_children l) <= summation size l) by auto using summation_flat_map.
+    auto with *.
+  Qed.
+
+  (** The general-purpose breadth-first search function. *)
+  Function find_generic (l:list finish) { measure l_size l } : option finish :=
+  match (List.find check l) with
+  | Some x => Some x
+  | None =>
+    let frontier := flat_map get_children l in
+    if is_nil frontier then None else find_generic frontier
+  end.
+  Proof.
+    intros.
+    auto using l_size_children_not_nil.
+  Qed.
+  
+  Lemma flat_map_get_children_rw_cons_ready:
+    forall t l1 l2,
+    flat_map get_children (Node ((t, Ready) :: l1) :: l2) =
+    flat_map get_children (Node l1 :: l2).
+  Proof.
+    intros.
+    simpl.
+    trivial.
+  Qed.
+    
+  (** A wrapper around [find_generic] that retrieves *)
+  Definition find (f:finish) := find_generic (f::nil).
+
+  Lemma find_generic_impl_check:
+    forall l f,
+    find_generic l = Some f ->
+    check f = true.
+  Proof.
+    intros.
+    functional induction (find_generic l).
+    - inversion H; subst; clear H.
+      induction l.
+      + inversion e.
+      + simpl in e.
+        remember (check a).
+        destruct b.
+        * inversion e; subst; auto.
+        * auto.
+    - inversion H.
+    - auto.
+  Qed.
+  
+  Lemma find_impl_check:
+    forall f f',
+    find f = Some f' ->
+    check f' = true.
+  Proof.
+    intros.
+    eauto using find_generic_impl_check.
+  Qed.
+
+  Lemma find_generic_nil:
+    find_generic nil = None.
+  Proof.
+    rewrite find_generic_equation.
+    auto.
+  Qed.
+
+  Require Import Coq.Relations.Relation_Operators.
+  
+  Lemma find_generic_impl_lt:
+    forall f l f',
+    Forall (fun f' => Lt f' f) l ->
+    find_generic l = Some f' ->
+    Lt f' f.
+  Proof.
+    intros f.
+    induction f using lt_ind.
+    - intros.
+      destruct l.
+      + rewrite find_generic_nil in H0; inversion H0.
+      + inversion H.
+        subst.
+        apply lt_leaf_absurd in H3.
+        inversion H3.
+    - intros.
+      apply lt_cons.
+      assert (Hx := IHf l0 f').
+      apply Hx; auto.
+      + rewrite Forall_forall in *.
+        intros.
+        eauto using lt_inv_cons_ready.
+    - intros.
+      unfold Lt.
+      apply t_trans.
+  Qed.
+
+  Lemma find_generic_contract:
+    forall t l1 l2 f,
+    find_generic (Node ((t, Ready) :: l1) :: l2) = Some f ->
+    check (Node ((t, Ready) :: l1)) = false ->
+    check (Node l1) = false ->
+    find_generic (Node l1 :: l2) = Some f.
+  Proof.
+    intros.
+    rewrite find_generic_equation in *.
+    rewrite flat_map_get_children_rw_cons_ready in H.
+    simpl in *.
+    rewrite H1.
+    rewrite H0 in H.
+    trivial.
+  Qed.
+
+  Lemma find_spec_1:
+    forall f f',
+    find f = Some f' ->
+    check f = false ->
+    Lt f' f /\ check f' = true.
+  Proof.
+    intros f.
+    unfold find.
+    induction f using finish_ind_strong.
+    - intros.
+      rewrite find_generic_equation in H.
+      simpl in H.
+      rewrite H0 in H.
+      inversion H.
+    - intros.
+      assert (Lt f' (Node l) /\ check f' = true). {
+        apply IHf.
+        + apply find_generic_contract with (t); auto.
+          
+      }*)
+      rewrite find_generic_equation in H.
+      rewrite H in *.
+      remember (is_nil _).
+      destruct b.
+      { inversion H. }
+      apply IHf in H.
+      } 
+      rewrite find_generic_equation in H.
+      simpl List.find in H.
+      rewrite H0 in H.
+      remember (flat_map _ _) as l'.
+      assert (l' = get_children (Node l)). {
+        subst.
+        simpl.
+        auto with *.
+      }
+      rewrite H1 in *.
+      remember (is_nil _).
+      destruct b.
+      { inversion H. }
+      apply IHf in H.
+End Find.
+
